Tried to make an executable definition. Kinda failed, but I still want to save this…

thy/AbstractBDD.thy
@@ -10,49 +10,129 @@ record abdd_node =
 	left :: nodelabel
 	
 record abdd =
-	nodes :: "abdd_node set"
+	nodes :: "abdd_node list"
 	start :: nodelabel
 
 definition abdd_reference_integrity_set :: "abdd \<Rightarrow> bool" where
-"abdd_reference_integrity_set b \<equiv> (\<forall>n \<in> nodes b.
-	(\<forall>m \<in> nodes b. (label m = label n) \<longrightarrow> (m = n)) \<and> (
+"abdd_reference_integrity_set b \<equiv> (\<forall>n \<in> set (nodes b).
+	(\<forall>m \<in> set (nodes b). (label m = label n) \<longrightarrow> (m = n)) \<and> (
 	case (label n) of 
-		LabeledNode _ \<Rightarrow> ((\<exists>l \<in> nodes b. label l = left n) \<and> (\<exists>l \<in> nodes b. label l = right n)) |
+		LabeledNode _ \<Rightarrow> ((\<exists>l \<in> set (nodes b). label l = left n) \<and> (\<exists>l \<in> set (nodes b). label l = right n)) |
 		_ \<Rightarrow> True))"
-definition "abdd_collect_refs bdd = {start bdd} \<union> right ` nodes bdd \<union> left ` nodes bdd"
+
+definition "abdd_collect_refs bdd = start bdd # map right (nodes bdd) @ map left (nodes bdd)"
 definition abdd_reference_integrity :: "abdd \<Rightarrow> bool" where
-	"abdd_reference_integrity bdd \<equiv> (\<forall>lb \<in> abdd_collect_refs bdd. \<exists>node \<in> nodes bdd. label node = lb)"
+	"abdd_reference_integrity bdd \<equiv> (\<forall>lb \<in> set (abdd_collect_refs bdd). \<exists>node \<in> set (nodes bdd). label node = lb)"
 definition abdd_nodes_unique :: "abdd \<Rightarrow> bool" where
-	"abdd_nodes_unique bdd \<equiv> (\<forall>n \<in> nodes bdd. (\<forall>m \<in> nodes bdd. (label m = label n) \<longrightarrow> (m = n)))"
-		
-definition "abddn_is_child c n \<equiv> (label c = left n \<or> label c = right n)" 
+	"abdd_nodes_unique bdd \<equiv> (\<forall>n \<in> set (nodes bdd). (\<forall>m \<in> set (nodes bdd). (label m = label n) \<longrightarrow> (m = n)))"
+
+definition "getnode bdd lbl = List.find (\<lambda>n. label n = lbl) (nodes bdd)"
+
+lemma getnode_noNone: "lbl \<in> set (abdd_collect_refs bdd) \<Longrightarrow> abdd_reference_integrity bdd \<Longrightarrow> getnode bdd lbl \<noteq> None"
+	unfolding abdd_reference_integrity_def getnode_def
+	unfolding find_None_iff
+	by blast
+	
+lemma node_gettable:
+	assumes "node \<in> set (nodes bdd)" and "abdd_reference_integrity bdd"
+	shows "getnode bdd (right node) \<noteq> None" "getnode bdd (left node) \<noteq> None"
+proof -
+	have "(right node) \<in> set (abdd_collect_refs bdd)" "(left node) \<in> set (abdd_collect_refs bdd)"
+		using assms unfolding abdd_reference_integrity_def abdd_collect_refs_def by auto
+	with getnode_noNone assms(2) show "getnode bdd (right node) \<noteq> None" "getnode bdd (left node) \<noteq> None" by simp_all
+qed
+lemma getnode_label_inv:
+	assumes "node \<in> set (nodes bdd)" and "abdd_reference_integrity bdd"
+	shows "label (the (getnode bdd (right node))) = right node" "label (the (getnode bdd (left node))) = left node"
+using node_gettable[OF assms] by simp_all (metis (mono_tags, lifting) find_Some_iff option.sel getnode_def)+
+lemma getnode_in:
+	assumes "node \<in> set (nodes bdd)" and "abdd_reference_integrity bdd"
+	shows "the (getnode bdd (right node)) \<in> set (nodes bdd)" "the (getnode bdd (left node)) \<in> set (nodes bdd)"
+using node_gettable[OF assms] by simp_all (metis find_Some_iff getnode_def nth_mem option.sel)+
+lemma getnode_in2: "getnode bdd (LabeledNode ln) = Some x \<Longrightarrow> x \<in> set (nodes bdd)"
+	unfolding getnode_def find_Some_iff by force
+
+definition "abdd_is_child c n \<equiv> (label c = left n \<or> label c = right n)"
 inductive abdd_reachable :: "abdd \<Rightarrow> abdd_node \<Rightarrow> abdd_node \<Rightarrow> bool" where
-ar_base: "ln2 \<in> nodes bdd \<Longrightarrow> abddn_is_child ln2 ln  \<Longrightarrow> abdd_reachable bdd ln ln2" |
-ar_step: "ln2 \<in> nodes bdd \<Longrightarrow> abdd_reachable bdd ln ln2 \<Longrightarrow> abddn_is_child ln3 ln2  \<Longrightarrow> abdd_reachable bdd ln ln3"
+ar_base: "ln2 \<in> set (nodes bdd) \<Longrightarrow> abdd_is_child ln2 ln  \<Longrightarrow> abdd_reachable bdd ln ln2" |
+ar_step: "ln3 \<in> set (nodes bdd) \<Longrightarrow> abdd_reachable bdd ln ln2 \<Longrightarrow> abdd_is_child ln3 ln2  \<Longrightarrow> abdd_reachable bdd ln ln3"
 code_pred abdd_reachable .
 definition "abdd_reachable_set bdd node = {n |n. abdd_reachable bdd node n}"
-definition "abdd_cycle_free bdd = (\<forall>node \<in> nodes bdd. \<not> abdd_reachable bdd node node)"
+definition "abdd_cycle_free bdd = (\<forall>node \<in> set (nodes bdd). \<not> abdd_reachable bdd node node)"
 
-definition abdd_is_dag :: "abdd \<Rightarrow> bool" where
-"abdd_is_dag bdd = (\<forall>n \<in> nodes bdd. \<not>abdd_reachable bdd n n)"
+lemma reachable_trans: "abdd_reachable bdd b c \<Longrightarrow> abdd_reachable bdd a b \<Longrightarrow> abdd_reachable bdd a c"
+	apply(induction rule: abdd_reachable.induct)
+	 apply(metis ar_step)+
+done
+lemma reachable_child: 
+	assumes "node \<in> set (nodes bdd)" "abdd_reference_integrity bdd"
+	shows "abdd_reachable bdd node (the (getnode bdd (right node)))" "abdd_reachable bdd node (the (getnode bdd (left node)))"
+proof -
+	have ic: "abdd_is_child (the (getnode bdd (right node))) node" "abdd_is_child (the (getnode bdd (left node))) node"
+		unfolding abdd_is_child_def using node_gettable[OF assms] getnode_label_inv[OF assms] by simp_all 
+	show "abdd_reachable bdd node (the (getnode bdd (right node)))" "abdd_reachable bdd node (the (getnode bdd (left node)))" using getnode_in[OF assms] ic ar_base by simp_all
+qed
+lemma step_reachable_subset_r: "node \<in> set (nodes bdd) \<Longrightarrow> abdd_reference_integrity bdd \<Longrightarrow> 
+       abdd_reachable_set bdd (the (getnode bdd (right node))) \<subseteq> (abdd_reachable_set bdd node)"
+proof(rule, unfold abdd_reachable_set_def, simp, fast elim: reachable_trans[OF _ reachable_child(1)]) qed
+lemma step_reachable_subset_l: "node \<in> set (nodes bdd) \<Longrightarrow> abdd_reference_integrity bdd \<Longrightarrow> 
+       abdd_reachable_set bdd (the (getnode bdd (left node))) \<subseteq> (abdd_reachable_set bdd node)"
+proof(rule, unfold abdd_reachable_set_def, simp, fast elim: reachable_trans[OF _ reachable_child(2)]) qed
 
-lemma "abdd_is_dag bdd \<Longrightarrow>
-       (*abdd_reference_integrity bdd \<Longrightarrow>*) 
-       abdd_reachable_set bdd (getnode bdd (right node)) \<subseteq> (abdd_reachable_set bdd node)"
-apply(rule, unfold abdd_reachable_set_def, simp)
-oops
+lemma hlp1: "x \<in> {n |n. P n} \<Longrightarrow> P x" by blast
+lemma notselfreach:
+	assumes "abdd_cycle_free bdd"
+	shows "node \<in> abdd_reachable_set bdd node \<Longrightarrow> False"
+proof(unfold abdd_reachable_set_def, drule hlp1)
+	case goal1
+	then have "node \<in> set (nodes bdd)" by(cases rule: abdd_reachable.cases) simp_all
+	moreover note assms[unfolded abdd_cycle_free_def]
+	ultimately show False using goal1 by simp
+qed
+lemma step_reachable_rsubset_l:
+	assumes a1: "abdd_cycle_free bdd"
+	assumes a2: "node \<in> set (nodes bdd)" "abdd_reference_integrity bdd"
+	shows "abdd_reachable_set bdd (the (getnode bdd (left node))) \<subset> (abdd_reachable_set bdd node)"
+	apply rule
+	 using step_reachable_subset_l[OF a2] apply simp
+	using notselfreach[OF a1] unfolding abdd_reachable_set_def using a2 mem_Collect_eq reachable_child(2) apply auto
+done
+lemma step_reachable_rsubset_r:
+	assumes a1: "abdd_cycle_free bdd"
+	assumes a2: "node \<in> set (nodes bdd)" "abdd_reference_integrity bdd"
+	shows "abdd_reachable_set bdd (the (getnode bdd (right node))) \<subset> (abdd_reachable_set bdd node)"
+	apply rule
+	 using step_reachable_subset_r[OF a2] apply simp
+	using notselfreach[OF a1] unfolding abdd_reachable_set_def using a2 mem_Collect_eq reachable_child(1) apply auto
+done
+
+lemma abdd_reachable_subset: "abdd_reachable_set bdd node \<subseteq> set (nodes bdd)"
+	apply(unfold abdd_reachable_set_def)
+	apply rule
+	apply(drule hlp1)
+	using abdd_reachable.simps apply blast
+done
+lemma abdd_reachable_fin: "finite (abdd_reachable_set bdd node)"
+	apply(rule finite_subset)
+	 apply(rule abdd_reachable_subset)
+	apply(rule finite_set)
+done
+
+lemma abdd_reachable_in_reachable:
+	"abdd_reachable bdd n1 n2 \<Longrightarrow> n2 \<in> abdd_reachable_set bdd n1"
+	unfolding abdd_reachable_set_def by simp
 
 definition "abdd_terminal state = (case state of LabeledNode _ \<Rightarrow> False | _ \<Rightarrow> True)" 
 
 inductive abdd_smallstep  where
 start: "abdd_smallstep bdd assignment (start bdd)" |
-step[elim]: "abdd_smallstep bdd assignment state \<Longrightarrow> \<not> abdd_terminal state \<Longrightarrow> node \<in> nodes bdd \<Longrightarrow> label node = state \<Longrightarrow> abdd_smallstep bdd assignment ((if assignment ! var node then right else left) node)"
+step[elim]: "abdd_smallstep bdd assignment state \<Longrightarrow> \<not> abdd_terminal state \<Longrightarrow> node \<in> set (nodes bdd) \<Longrightarrow> label node = state \<Longrightarrow> abdd_smallstep bdd assignment ((if assignment ! var node then right else left) node)"
 print_theorems
 code_pred abdd_smallstep .
 inductive abdd_smallstep2  where
 start: "abdd_smallstep2 bdd assignment (start bdd)" |
-stepright: "abdd_smallstep2 bdd assignment state \<Longrightarrow> \<not> abdd_terminal state \<Longrightarrow> node \<in> nodes bdd \<Longrightarrow> label node = state \<Longrightarrow> assignment ! var node \<Longrightarrow> abdd_smallstep2 bdd assignment (right node)" |
-stepleft: "abdd_smallstep2 bdd assignment state \<Longrightarrow> \<not> abdd_terminal state \<Longrightarrow> node \<in> nodes bdd \<Longrightarrow> label node = state \<Longrightarrow> \<not>assignment ! var node \<Longrightarrow> abdd_smallstep2 bdd assignment (left node)"
+stepright: "abdd_smallstep2 bdd assignment state \<Longrightarrow> \<not> abdd_terminal state \<Longrightarrow> node \<in> set (nodes bdd) \<Longrightarrow> label node = state \<Longrightarrow> assignment ! var node \<Longrightarrow> abdd_smallstep2 bdd assignment (right node)" |
+stepleft: "abdd_smallstep2 bdd assignment state \<Longrightarrow> \<not> abdd_terminal state \<Longrightarrow> node \<in> set (nodes bdd) \<Longrightarrow> label node = state \<Longrightarrow> \<not>assignment ! var node \<Longrightarrow> abdd_smallstep2 bdd assignment (left node)"
 lemma abdd_smallstep_2_eq: "abdd_smallstep bdd ass state = abdd_smallstep2 bdd ass state"
 	apply(rule)
 	 apply(induction rule: abdd_smallstep.induct)
@@ -64,25 +144,25 @@ lemma abdd_smallstep_2_eq: "abdd_smallstep bdd ass state = abdd_smallstep2 bdd a
 	apply(force dest: abdd_smallstep.step)
 done
 
-definition "abdd_xor \<equiv> \<lparr> nodes = {
+definition "abdd_xor \<equiv> \<lparr> nodes = [
 	\<lparr> var = 0, label = LabeledNode 5, right = LabeledNode 4 , left = LabeledNode 3 \<rparr>,
 	\<lparr> var = 1, label = LabeledNode 4, right = DFalse , left = DTrue \<rparr>,
 	\<lparr> var = 1, label = LabeledNode 3, right = DTrue , left = DFalse \<rparr>,
 	\<lparr> var = 0, label = DTrue , right = DTrue , left = DTrue \<rparr>,
 	\<lparr> var = 0, label = DFalse , right = DFalse , left = DFalse \<rparr>
-}, start = LabeledNode 5\<rparr>"
+], start = LabeledNode 5\<rparr>"
 
-lemma "abdd_reference_integrity abdd_xor" by eval
-lemma "abdd_cycle_free abdd_xor" unfolding abdd_cycle_free_def apply(subst abdd_xor_def, simp) apply(rule) oops 
+lemma "abdd_reference_integrity abdd_xor = True" by eval
+lemma[code]: "abdd_cycle_free abdd_xor = True" 
+unfolding abdd_cycle_free_def eq_True apply(subst abdd_xor_def, simp) apply(rule) oops
 lemma "abdd_smallstep abdd_xor [False, True] DTrue" 
 proof -
 	have 1: "abdd_smallstep abdd_xor [False, True] (start abdd_xor)" by(simp add: abdd_smallstep.start)
-	have 2: "\<lparr> var = 0, label = LabeledNode 5, right = LabeledNode 4 , left = LabeledNode 3 \<rparr> \<in> nodes abdd_xor" by(simp add: abdd_xor_def)
+	have 2: "\<lparr> var = 0, label = LabeledNode 5, right = LabeledNode 4 , left = LabeledNode 3 \<rparr> \<in> set (nodes abdd_xor)" by(simp add: abdd_xor_def)
 	have 3: "abdd_smallstep abdd_xor [False, True] (LabeledNode 3)" using abdd_smallstep.step[OF 1 _ 2] by(simp add: abdd_xor_def abdd_terminal_def)
-	have 4: "\<lparr> var = 1, label = LabeledNode 3, right = DTrue , left = DFalse \<rparr> \<in> nodes abdd_xor" by(simp add: abdd_xor_def)
+	have 4: "\<lparr> var = 1, label = LabeledNode 3, right = DTrue , left = DFalse \<rparr> \<in> set (nodes abdd_xor)" by(simp add: abdd_xor_def)
 	show 5: "abdd_smallstep abdd_xor [False, True] DTrue" using abdd_smallstep.step[OF 3 _ 4] by(simp add: abdd_xor_def abdd_terminal_def)
-qed (* So how do I do this automatically? *)
-values "{t|t. abdd_smallstep2 abdd_xor [False, True] t}" (* I guess I don't? *)
+qed (* So how do I do this automatically? Guess I don't *)
 
 definition "abstract_abdd1 bdd ass = (
 	if abdd_smallstep bdd ass DTrue
@@ -91,14 +171,182 @@ definition "abstract_abdd1 bdd ass = (
 		then Some False
 	else None))"
 
-lemma abdd_steppable_ind: " (\<exists>node \<in> nodes bdd. label node = state)
-	\<Longrightarrow> abdd_smallstep bdd ass state \<Longrightarrow> (\<exists>nextnode \<in> nodes bdd. abdd_smallstep bdd ass (label nextnode))" by blast
+lemma abdd_steppable_ind: " (\<exists>node \<in> set (nodes bdd). label node = state)
+	\<Longrightarrow> abdd_smallstep bdd ass state \<Longrightarrow> (\<exists>nextnode \<in> set (nodes bdd). abdd_smallstep bdd ass (label nextnode))" by blast
 
+function abstract_abdd2 :: "abdd \<Rightarrow> nodelabel \<Rightarrow> boolfunc2" where
+"abstract_abdd2 bdd DTrue = (\<lambda>as. True)" |
+"abstract_abdd2 bdd DFalse = (\<lambda>as. False)" |
+"abstract_abdd2 bdd (LabeledNode ln) = (if abdd_reference_integrity bdd \<and> abdd_cycle_free bdd then 
+	(case getnode bdd (LabeledNode ln) of Some n \<Rightarrow> 
+		(\<lambda>as. if as (var n) then abstract_abdd2 bdd (right n) as 
+		else abstract_abdd2 bdd (left n) as)
+		| _ \<Rightarrow> undefined) else undefined)"
+by pat_completeness auto
 
-lemma "abdd_reference_integrity bdd \<Longrightarrow> abdd_cycle_free bdd \<Longrightarrow> abstract_abdd1 bdd ass \<noteq> None"
-apply(unfold abstract_abdd1_def)
-apply(unfold abdd_smallstep_2_eq)
+termination abstract_abdd2
+proof(relation "measure (\<lambda>(bdd, nl). case getnode bdd nl of Some n \<Rightarrow> card (abdd_reachable_set bdd n) | None \<Rightarrow> 0)", rule wf_measure)
+	case goal1
+	then have as: "abdd_reference_integrity bdd" "abdd_cycle_free bdd" by simp_all
+	have xe: "x2 \<in> set (nodes bdd)" using getnode_in2[OF goal1(2)] . 
+	have cs: "(case getnode bdd (right x2) of None \<Rightarrow> 0 | Some n \<Rightarrow> card (abdd_reachable_set bdd n)) =
+		card (abdd_reachable_set bdd  (the (getnode bdd (right x2))))" using node_gettable(1)[OF xe as(1)] by force
+	note psubset_card_mono[OF abdd_reachable_fin step_reachable_rsubset_r[OF as(2) xe as(1)]]
+	then show ?case by(simp add: cs goal1(2))
+next
+	case goal2
+	then have as: "abdd_reference_integrity bdd" "abdd_cycle_free bdd" by simp_all
+	have xe: "x2 \<in> set (nodes bdd)" using getnode_in2[OF goal2(2)] . 
+	have cs: "(case getnode bdd (left x2) of None \<Rightarrow> 0 | Some n \<Rightarrow> card (abdd_reachable_set bdd n)) =
+		card (abdd_reachable_set bdd  (the (getnode bdd (left x2))))" using node_gettable(2)[OF xe as(1)] by force
+	note psubset_card_mono[OF abdd_reachable_fin step_reachable_rsubset_l[OF as(2) xe as(1)]]
+	then show ?case by(simp add: cs goal2(2))
+qed
+
+(* I want to try a few examples\<dots> So I need something that can execude. *)
+function abdd_reachable_set_code where
+"abdd_reachable_set_code bdd nods = (if abdd_reference_integrity bdd then 
+	(let trunc = set (nodes bdd) \<inter> nods in (let morereach = trunc 
+		\<union> (the \<circ> getnode bdd \<circ> right) ` trunc
+		\<union> (the \<circ> getnode bdd \<circ> left) ` trunc in 
+			(if nods \<subset> morereach 
+			then abdd_reachable_set_code bdd morereach 
+			else trunc)))
+	else undefined)"
+by pat_completeness auto
+termination abdd_reachable_set_code
+proof(relation "measure (\<lambda>(bdd,nods). length (nodes bdd) - card nods)", rule wf_measure, unfold comp_def)
+	case goal1
+	note xa = goal1(3)[unfolded goal1(2)]
+	note a = goal1(4)[unfolded xa]
+	have ss1: "x \<subseteq> set (nodes bdd)" unfolding goal1(2) by simp
+	then have ss2: "xa \<subseteq> set (nodes bdd)" unfolding goal1(3)
+		by(auto simp add: getnode_in[OF _ goal1(1)])
+	have lep1: "card xa \<le> length (nodes bdd)"
+		using le_trans card_mono[OF finite_set ss2, unfolded card_set] length_remdups_leq .
+	have lep2: "card nods \<le> length (nodes bdd)"
+		 by (meson List.finite_set card_mono finite_subset goal1(4) le_trans lep1 less_imp_le ss2)
+	{ fix x y z :: nat
+		have "y \<le> x \<Longrightarrow> z \<le> x \<Longrightarrow> x - y < x - z = (z < y)" by linarith
+	} note swapdir = this
+	show ?case unfolding in_measure
+		by(simp add: swapdir[OF lep1 lep2] psubset_card_mono[OF _ a, simplified, unfolded xa[symmetric]])
+qed
+print_theorems
+
+lemma reachable_code_subset_self: 
+	"x \<subseteq> set (nodes bdd) \<Longrightarrow> abdd_reference_integrity bdd \<Longrightarrow> x \<subseteq> abdd_reachable_set_code bdd x"
+proof(induction bdd x rule: abdd_reachable_set_code.induct)
+	case goal1
+	let ?trunc = "set (nodes bdd) \<inter> nods"
+	let ?morereach = "?trunc \<union> (the \<circ> getnode bdd \<circ> right) ` ?trunc \<union> (the \<circ> getnode bdd \<circ> left) ` ?trunc"
+	note mih = goal1(1)[OF goal1(3) _ _ _ _ goal1(3), of ?trunc ?morereach, OF refl refl]
+	have "?morereach \<subseteq> set (nodes bdd)" using goal1(2) unfolding comp_def using getnode_in[OF _ goal1(3)] by blast
+	note fih = mih[OF _ this]
+	have df: "abdd_reachable_set_code bdd nods =  
+		(if nods \<subset> ?morereach then abdd_reachable_set_code bdd ?morereach else ?trunc)"
+		using goal1(3) by(simp add: Let_def) 
+	show ?case proof(cases "nods \<subset> ?morereach")
+		case False show ?thesis unfolding df[unfolded if_not_P[OF False]] using goal1(2) by simp
+	next
+		case True
+		note fih[OF True]
+		thus ?thesis using df[unfolded if_P[OF True]] using goal1(2) by blast
+	qed
+qed
+
+lemma reach_eq_hlp1: "abdd_reference_integrity bdd \<Longrightarrow> ln2 \<in> abdd_reachable_set_code bdd ln \<Longrightarrow>
+	abdd_is_child ln3 ln2 \<Longrightarrow> ln3 \<in> set (nodes bdd) \<Longrightarrow> ln3 \<in> abdd_reachable_set_code bdd ln"
+apply(auto simp only: abdd_is_child_def)
+apply(subst abdd_reachable_set_code.simps, subst abdd_reachable_set_code.simps)
+sorry
+
+lemma reach_eq_help2: "abdd_reference_integrity bdd \<Longrightarrow> \<Union>(abdd_reachable_set bdd `
+         (set (nodes bdd) \<inter> nods \<union> (the \<circ> getnode bdd \<circ> right) ` (set (nodes bdd) \<inter> nods) \<union>
+          (the \<circ> getnode bdd \<circ> left) ` (set (nodes bdd) \<inter> nods))) \<union>
+       (set (nodes bdd) \<inter> nods \<union> (the \<circ> getnode bdd \<circ> right) ` (set (nodes bdd) \<inter> nods) \<union>
+        (the \<circ> getnode bdd \<circ> left) ` (set (nodes bdd) \<inter> nods)) = 
+          \<Union>(abdd_reachable_set bdd ` (set (nodes bdd) \<inter> nods)) \<union> (set (nodes bdd) \<inter> nods)"
+proof
+	case goal1
+	have r2: "\<Union>(abdd_reachable_set bdd ` (the \<circ> getnode bdd \<circ> right) ` (set (nodes bdd) \<inter> nods))
+    	\<subseteq> \<Union>(abdd_reachable_set bdd ` (set (nodes bdd) \<inter> nods))"
+    	by(rule, unfold image_comp comp_def) (blast dest: step_reachable_subset_r[OF _ goal1])
+    have l2: "\<Union>(abdd_reachable_set bdd ` (the \<circ> getnode bdd \<circ> left) ` (set (nodes bdd) \<inter> nods))
+    	\<subseteq> \<Union>(abdd_reachable_set bdd ` (set (nodes bdd) \<inter> nods))"
+    	by(rule, unfold image_comp comp_def) (blast dest: step_reachable_subset_l[OF _ goal1])
+    have m: "(the \<circ> getnode bdd \<circ> right) ` (set (nodes bdd) \<inter> nods) \<union>
+    	(the \<circ> getnode bdd \<circ> left) ` (set (nodes bdd) \<inter> nods) \<subseteq> \<Union>(abdd_reachable_set bdd ` (set (nodes bdd) \<inter> nods))"
+    	using abdd_reachable_in_reachable reachable_child[OF _ goal1] by auto
+	show ?case
+		using l2 r2 m
+		unfolding image_Un
+		by auto
+qed force
+
+lemma subset_hlp: "({x} \<subseteq> S) = (x \<in> S)" by simp
+lemma abdd_reachable_set_code_eq_hlp: "abdd_reference_integrity bdd \<Longrightarrow> node \<in> set (nodes bdd) \<Longrightarrow>
+	abdd_reachable_set_code bdd {node} = abdd_reachable_set bdd node \<union> {node}"
+proof
+	case goal2 have "abdd_reachable_set bdd node \<subseteq> abdd_reachable_set_code bdd {node}"
+		(* Caesar style proof: no facts written. *) 
+		apply(rule)
+		apply(unfold abdd_reachable_set_def) 
+		apply(drule hlp1)
+		using goal2 proof -
+			case goal1 thus ?case proof(induction rule: abdd_reachable.induct)
+				case goal1
+				from reach_eq_hlp1[OF goal1(3) _ goal1(2) goal1(1), of "{ln}"]
+					reachable_code_subset_self[of "{ln}", unfolded subset_hlp, OF goal1(4) goal1(3)]
+				show ?case .
+			next
+				case goal2 (* with reach_eq_hlp1 show ?case by blast *)
+				note mih = goal2(3)[OF goal2(5) goal2(6)]
+				note reach_eq_hlp1[OF goal2(5) mih goal2(4) goal2(1)]
+				thus ?case .
+			qed
+		qed
+	then show ?case
+		using reachable_code_subset_self[OF goal2(2)[unfolded subset_hlp[symmetric]] goal2(1)]
+		by simp
+next
+	case goal1
+	{ fix k e
+		have "e \<in> abdd_reachable_set_code bdd k \<Longrightarrow> e \<in> \<Union>(abdd_reachable_set bdd ` k) \<union> k"
+		using goal1
+		proof(induction bdd k rule: abdd_reachable_set_code.induct)
+			case goal1
+			let ?trunc = "set (nodes bdd) \<inter> nods"
+			let ?morereach = "?trunc \<union> (the \<circ> getnode bdd \<circ> right) ` ?trunc \<union> (the \<circ> getnode bdd \<circ> left) ` ?trunc"
+			note mih = goal1(1)[OF goal1(3), of ?trunc ?morereach, OF refl refl _ _ goal1(3) goal1(4)]
+			have df: "abdd_reachable_set_code bdd nods =  
+				(if nods \<subset> ?morereach then abdd_reachable_set_code bdd ?morereach else ?trunc)"
+				using goal1(3) by(simp add: Let_def) 
+			thus ?case (is ?kees) 
+			proof(cases "nods \<subset> ?morereach")
+				case True
+				note mdf = df[unfolded if_P[OF True], symmetric]
+				from mih[OF True]
+				show ?kees unfolding mdf unfolding reach_eq_help2[OF goal1(3)]
+					using goal1(2) by blast
+			next
+				case False
+				note mdf = df[unfolded if_not_P[OF False]]
+				show ?kees using goal1(2)[unfolded mdf] by blast
+			qed
+		qed
+			
+	}
+	from this[of _ "{node}"] show ?case by blast
+qed
+
+lemma [code]: "(if abdd_reference_integrity bdd \<and> abdd_cycle_free bdd then a else b) =
+               (if abdd_reference_integrity bdd \<and> (\<forall>node \<in> set (nodes bdd). 
+               		node \<notin> abdd_reachable_set_code bdd node) then a else b)"
+using abdd_reachable_set_code_eq_hlp
+
+lemma abdd_reachable_dub: assumes "abdd_reference_integrity bdd" "nod \<in> set (nodes bdd)"
+	shows "\<Union>(abdd_reachable_set bdd ` abdd_reachable_set bdd nod) = abdd_reachable_set bdd nod"
 oops
-
-
+	
 end
